@prefix cc:    <http://creativecommons.org/ns#> .
@prefix void:  <http://rdfs.org/ns/void#> .
@prefix ecc:   <https://ns.eccenca.com/> .
@prefix owl:   <http://www.w3.org/2002/07/owl#> .
@prefix xsd:   <http://www.w3.org/2001/XMLSchema#> .
@prefix skos:  <http://www.w3.org/2004/02/skos/core#> .
@prefix voaf:  <http://purl.org/vocommons/voaf#> .
@prefix mv:    <http://schema.mobivoc.org/> .
@prefix dbpedia: <http://dbpedia.org/resource/> .
@prefix rdfs:  <http://www.w3.org/2000/01/rdf-schema#> .
@prefix vcard: <http://www.w3.org/2001/vcard-rdf/3.0#> .
@prefix gr:    <http://purl.org/goodrelations/v1#> .
@prefix dbo:   <http://dbpedia.org/> .
@prefix geo:   <http://www.w3.org/2003/01/geo/wgs84_pos#> .
@prefix s:     <http://schema.org/> .
@prefix dct:   <http://purl.org/dc/terms/> .
@prefix doap:  <http://usefulinc.com/ns/doap#> .
@prefix rdf:   <http://www.w3.org/1999/02/22-rdf-syntax-ns#> .
@prefix vann:  <http://purl.org/vocab/vann/> .
@prefix foaf:  <http://xmlns.com/foaf/0.1/> .

mv:entrance  a            owl:ObjectProperty , rdf:Property ;
        rdfs:comment      "Describes the entrance of a parking facility."@en ;
        rdfs:domain       mv:ParkingFacility ;
        rdfs:isDefinedBy  mv: ;
        rdfs:label        "hat Einfahrt"@de , "entrance"@en ;
        rdfs:range        mv:ParkingFacilityEntrance .

mv:chargingPoint  a       owl:ObjectProperty , rdf:Property ;
        rdfs:comment      "Indicates whether charging points are available." ;
        rdfs:domain       [ a            owl:Class ;
                            owl:unionOf  ( mv:ParkingFacility mv:ParkingSpace )
                          ] ;
        rdfs:isDefinedBy  mv: ;
        rdfs:label        "hat Ladestation"@de , "has charging point"@en ;
        rdfs:range        mv:ChargingPoint .

mv:CEE_7_4  a               mv:PlugType ;
        rdfs:comment        "The CEE 7/3 socket and CEE 7/4 plug are commonly called Schuko. The socket (which is often, in error, also referred to as CEE 7/4) has a predominantly circular recess which is 17.5 mm (0.689 in) deep with two symmetrical round apertures and two earthing clips on the sides of the socket positioned to ensure that the earth is always engaged before live pin contact is made. The plug pins are 4.8 by 19 mm (0.189 by 0.748 in)." ;
        rdfs:isDefinedBy    mv: ;
        rdfs:label          "CEE 7/4"@en ;
        rdfs:seeAlso        <https://en.wikipedia.org/wiki/AC_power_plugs_and_sockets#CEE_7/5_socket_and_CEE_7/6_plug_(French;_Type_E)> ;
        mv:ocmConnectionID  "28" ;
        skos:altLabel       "Type F" , "Schuko" ;
        foaf:depiction      <https://upload.wikimedia.org/wikipedia/commons/e/ef/Schuko_plug_and_socket.png> .

mv:UndergroundParkingGarage
        a                 rdfs:Class , owl:Class ;
        rdfs:comment      "Parking facility with one or more levels below the surface and none above ground." ;
        rdfs:isDefinedBy  mv: ;
        rdfs:label        "Tiefgarage"@de , "Underground parking garage"@en ;
        rdfs:subClassOf   mv:ParkingFacility ;
        skos:altLabel     "Rampengarage"@de ;
        skos:prefLabel    "Tiefgarage"@de , "Underground parking garage"@en .

s:Place  a                owl:Class ;
        rdfs:comment      "Entities that have a somewhat fixed, physical extension."@en ;
        rdfs:isDefinedBy  s: ;
        rdfs:label        "Place"@en .

mv:Faulty  a              mv:CivicStructureStatus ;
        rdfs:comment      "The parking facility is not operating normally." ;
        rdfs:isDefinedBy  mv: ;
        rdfs:label        "Faulty"@en , "Defekt"@de .

mv:level  a               owl:DatatypeProperty , rdf:Property ;
        rdfs:comment      "Indicates the level of a parking facility the parking space is located in."@en ;
        rdfs:domain       mv:ParkingSpace ;
        rdfs:isDefinedBy  mv: ;
        rdfs:label        "Ebene"@de , "level"@en ;
        rdfs:range        xsd:integer .

ecc:aweilandt  a   foaf:Person , dct:Agent ;
        foaf:name  "Annette Weilandt" .

mv:RecreationalVehicle
        a                 s:Vehicle ;
        rdfs:comment      "A motor vehicle or trailer equipped with living space and amenities found in a home."@en ;
        rdfs:isDefinedBy  mv: ;
        rdfs:label        "Wohnmobil"@de , "Recreational vehicle"@en .

s:address  a              owl:ObjectProperty ;
        rdfs:comment      "Physical address of the item."@en ;
        rdfs:domain       s:Place ;
        rdfs:isDefinedBy  s: ;
        rdfs:label        "address"@en ;
        rdfs:range        s:PostalAddress .

cc:license  a             owl:AnnotationProperty ;
        rdfs:isDefinedBy  <http://creativecommons.org/ns> .

mv:operatedBy  a          owl:ObjectProperty , rdf:Property ;
        rdfs:comment      "The operator of a civic structure or facility. Operator and owner can be different business entitites."@en ;
        rdfs:domain       s:CivicStructure ;
        rdfs:isDefinedBy  mv: ;
        rdfs:label        "betrieben von"@de , "operated by"@en ;
        rdfs:range        gr:BusinessEntity .

mv:ParkAndRide  a         mv:ParkingFacilityConnection ;
        rdfs:comment      "Connection to public transport." ;
        rdfs:isDefinedBy  mv: ;
        rdfs:label        "Parken und Reisen"@de , "Park & Ride"@en ;
        skos:altLabel     "P+R" , "P&R" .

mv:dueForTime  a          owl:ObjectProperty , rdf:Property ;
        rdfs:comment      "Indicates that a price specification is due for a certain time specification."@en ;
        rdfs:domain       s:PriceSpecification ;
        rdfs:isDefinedBy  mv: ;
        rdfs:label        "fällig für Zeitdauer"@de , "due for time"@en ;
        rdfs:range        mv:TimeSpecification .

mv:vehicleWidthLimitInM
        a                 owl:DatatypeProperty , rdf:Property ;
        rdfs:comment      "Indicates the width limit in meter for vehicles using the parking facility." ;
        rdfs:domain       s:CivicStructure ;
        rdfs:isDefinedBy  mv: ;
        rdfs:label        "Breitenbegrenzung für Fahrzeuge"@de , "vehicle width limit"@en ;
        rdfs:range        xsd:decimal .

mv:ParkAndRideServiceOperating
        a                 mv:CivicStructureStatus ;
        rdfs:comment      "Park and ride services are operating until the specified time." ;
        rdfs:isDefinedBy  mv: ;
        rdfs:label        "Park and ride service operating"@en , "P+R-Service vorhanden"@de .

mv:price  a               owl:ObjectProperty , rdf:Property ;
        rdfs:comment      "Indicates that a civic structure can be used for a specific price."@en ;
        rdfs:domain       s:CivicStructure ;
        rdfs:isDefinedBy  mv: ;
        rdfs:label        "Preis"@de , "price"@en ;
        rdfs:range        s:PriceSpecification .

ecc:eccenca-GmbH  a  foaf:Organization , dct:Agent ;
        foaf:name  "eccenca GmbH" .

mv:IEC_60309_3-pin  a       mv:PlugType ;
        rdfs:comment        "IEC 60309 (formerly IEC 309 and CEE 17, also published by CENELEC as EN 60309) is an international standard from the International Electrotechnical Commission (IEC) for \"plugs, socket-outlets and couplers for industrial purposes\". 3-Pin connector." ;
        rdfs:isDefinedBy    mv: ;
        rdfs:label          "IEC_60309 3-pin"@en ;
        rdfs:seeAlso        <https://en.wikipedia.org/wiki/IEC_60309> ;
        mv:ocmConnectionID  "34" , "16" .

mv:Carpooling  a          mv:ParkingFacilityConnection ;
        rdfs:comment      "Parking facility used for carpooling or ridesharing." ;
        rdfs:isDefinedBy  mv: ;
        rdfs:label        "Parken und Mitfahren"@de , "Carpooling" ;
        skos:altLabel     "Parken und Mitnehmen"@de , "Park & Drive" , "P+M" , "P&M" .

mv:access  a              owl:ObjectProperty , rdf:Property ;
        rdfs:comment      "Indicates that a civic structure can only be accessed when certain conditions are fullfilled."@en ;
        rdfs:domain       s:CivicStructure ;
        rdfs:isDefinedBy  mv: ;
        rdfs:label        "access"@en ;
        rdfs:range        mv:AccessCondition .

mv:currentValue  a        owl:DatatypeProperty , rdf:Property ;
        rdfs:comment      "Indicates the current value of the real-time capacity."@en ;
        rdfs:domain       mv:RealTimeCapacity ;
        rdfs:isDefinedBy  mv: ;
        rdfs:label        "current value"@en ;
        rdfs:range        xsd:integer .

mv:AS_3112_Type_I  a        mv:PlugType ;
        rdfs:comment        "AS/NZS 3112 are the harmonised Australian and New Zealand standards for AC Plugs and Socket-Outlets." ;
        rdfs:isDefinedBy    mv: ;
        rdfs:label          "AS 3112 Type I"@en ;
        rdfs:seeAlso        <https://en.wikipedia.org/wiki/AS/NZS_3112> ;
        mv:ocmConnectionID  "29" ;
        skos:altLabel       "Type I/AS 3112/CPCS-CCC" , "Type I" ;
        foaf:depiction      <https://upload.wikimedia.org/wikipedia/commons/thumb/2/20/Aust_AC_plug.jpg/800px-Aust_AC_plug.jpg> .

mv:charger  a             owl:ObjectProperty , rdf:Property ;
        rdfs:comment      "Describes the charger available at a charging point. A charging point can have more than one charger." ;
        rdfs:domain       mv:ChargingPoint ;
        rdfs:isDefinedBy  mv: ;
        rdfs:label        "charger"@en ;
        rdfs:range        mv:Charger .

mv:ElectricVehicle  a     s:Vehicle ;
        rdfs:comment      "A wheeled, self-powered motor vehicle using an electric drivetrain."@en ;
        rdfs:isDefinedBy  mv: ;
        rdfs:label        "Véhicule électrique"@fr , "Electric vehicle"@en , "Elektrofahrzeug"@de .

mv:ParallelParking  a     mv:ArrangementPattern ;
        rdfs:comment      "Bei der Längsaufstellung wird das Fahrzeug (gemäß § 12 StVO) parallel zur Fahrbahn geparkt. Diese Fahrzeugaufstellung ist die gängigste Aufstellungsart an Straßen."@de , "With parallel parking, vehicles are arranged in a line, with the front of one vehicle facing the back of an adjacent one. This is done parallel to a curb, when one is provided. Parallel parking is the most common mode of roadside parking for vehicles."@en ;
        rdfs:isDefinedBy  mv: ;
        rdfs:label        "Längsaufstellung"@de , "Parallel parking"@en ;
        skos:altLabel     "Parallelaufstellung"@de ;
        skos:prefLabel    "Längsaufstellung"@de , "Parallel parking"@en .

mv:ChargingPoint  a       owl:Class , rdfs:Class ;
        rdfs:comment      "Civic structure that supplies electric energy for the recharging of electric vehicles." ;
        rdfs:isDefinedBy  mv: ;
        rdfs:label        "Ladestation"@de , "Charging point"@en ;
        rdfs:subClassOf   s:CivicStructure .

mv:freeOfCharge  a        owl:DatatypeProperty , rdf:Property ;
        rdfs:comment      "Indicates that the usage of the civic structure is for free." ;
        rdfs:domain       s:PriceSpecification ;
        rdfs:isDefinedBy  mv: ;
        rdfs:label        "kostenlos"@de , "free of charge"@en ;
        rdfs:range        xsd:boolean .

mv:plug  a                owl:ObjectProperty , rdf:Property ;
        rdfs:comment      "Indicates the plugs available at a charger." ;
        rdfs:domain       mv:Charger ;
        rdfs:isDefinedBy  mv: ;
        rdfs:label        "plug"@en ;
        rdfs:range        mv:Plug .

mv:IEC_60309_16A_2_E  a     mv:PlugType ;
        rdfs:comment        "IEC 60309 (formerly IEC 309 and CEE 17, also published by CENELEC as EN 60309) is an international standard from the International Electrotechnical Commission (IEC) for \"plugs, socket-outlets and couplers for industrial purposes\". The blue P+N+E, 6h (180°) plug is a single phase connector. In particular this smallest (16 A) variant has become especially common in camping vehicles and sockets found in caravan parks and marinas throughout Europe." ;
        rdfs:isDefinedBy    mv: ;
        rdfs:label          "IEC_60309 16A 2+E"@en ;
        rdfs:seeAlso        <https://en.wikipedia.org/wiki/IEC_60309> ;
        mv:ocmConnectionID  "4" ;
        skos:altLabel       "Blue Commando (2P+E)" ;
        foaf:depiction      <https://upload.wikimedia.org/wikipedia/commons/thumb/c/c0/CEE_16A_230V_Wandsteckdose_Pinning.png/800px-CEE_16A_230V_Wandsteckdose_Pinning.png> .

mv:brand  a               owl:DatatypeProperty , rdf:Property ;
        rdfs:comment      "Indicates the brand of a charger." ;
        rdfs:domain       mv:Charger ;
        rdfs:isDefinedBy  mv: ;
        rdfs:label        "brand"@en , "Marke"@de ;
        rdfs:range        xsd:string .

mv:PlugType  a            owl:Class , rdfs:Class ;
        rdfs:comment      "Type of a plug that is used to connect electric vehicles." ;
        rdfs:isDefinedBy  mv: ;
        rdfs:label        "Steckertyp"@de , "Plug type"@en .

mv:IEC_62196_Type_3A  a     mv:PlugType ;
        rdfs:comment        "The type 3A is derived from the Scame charging connectors adding the IEC 62196 pins which is suited for single-phase charging – the connector builds on the experience with the Scame connector for charging of light vehicles (electric motorcycles and scooters)." ;
        rdfs:isDefinedBy    mv: ;
        rdfs:label          "SCAME Type 3A"@en ;
        rdfs:seeAlso        <https://en.wikipedia.org/wiki/IEC_62196#Type_3_(EV_Plug_Alliance_connector),_Scame> ;
        mv:ocmConnectionID  "36" ;
        skos:altLabel       "IEC 62196-2 Type 3A" .

mv:Women  a               mv:UserGroup ;
        rdfs:comment      "Female persons."@en ;
        rdfs:isDefinedBy  mv: ;
        rdfs:label        "Frauen"@de , "Women"@en .

mv:CEE_7_16  a              mv:PlugType ;
        rdfs:comment        "The CEE 7/16 standard sheet appears in Supplement 2 (June 1962) to the 1951 edition of CEE 7. The CEE 7/16 unearthed plug is used for low power Class II applications, it has two round 4 by 19 mm (0.157 by 0.748 in) pins, rated at 2.5 A. There are two variants." ;
        rdfs:isDefinedBy    mv: ;
        rdfs:label          "CEE 7/16"@en ;
        rdfs:seeAlso        <https://en.wikipedia.org/wiki/AC_power_plugs_and_sockets#CEE_7/16_plugs> ;
        mv:ocmConnectionID  "13" ;
        skos:altLabel       "Europlug" ;
        foaf:depiction      <https://upload.wikimedia.org/wikipedia/commons/6/63/Euro-Flachstecker_2.jpg> .

mv:Allow  a               mv:Action ;
        rdfs:comment      "Allow to do an action."@en ;
        rdfs:isDefinedBy  mv: ;
        rdfs:label        "Erlauben"@de , "Allow"@en .

mv:NoParkAndRideInformation
        a                 mv:CivicStructureStatus ;
        rdfs:comment      "No park and ride information will be available until the specified time." ;
        rdfs:isDefinedBy  mv: ;
        rdfs:label        "No park and ride information"@en , "Keine P+R-Informationen"@de .

gr:BusinessEntity  a      owl:class ;
        rdfs:comment      "An instance of this class represents the legal agent making (or seeking) a particular offering. This can be a legal body or a person. A business entity has at least a primary mailing address and contact details. For this, typical address standards (vCard) and location data (geo, WGS84) can be attached. Note that the location of the business entity is not necessarily the location from which the product or service is being available."@en ;
        rdfs:isDefinedBy  gr: ;
        rdfs:label        "Juristische Person"@de , "Business entity"@en .

mv:civicStructureStatus
        a                 owl:ObjectProperty , rdf:Property ;
        rdfs:comment      "Indicates the current status of the civil structure." ;
        rdfs:domain       s:CivicStructure ;
        rdfs:isDefinedBy  mv: ;
        rdfs:label        "hat Status der zivilen Struktur"@de , "civic structure status"@en ;
        rdfs:range        mv:CivicStructureStatus .

mv:     a                              owl:Ontology , voaf:Vocabulary ;
        rdfs:comment                   "Our goal is to significantly improve the data mobility between all stakeholders by providing a standardized vocabulary using Semantic Web technologies and ontologies. For the open vocabulary covering various mobility aspects we use RDF (Resource Description Framework) - a recommended specification of the World Wide Web Consortium (W3C) and the so-called lingua franca for the integration of data and web. We invite everyone who is interested to join our MobiVoc initiative and to participate in the development of the Open Mobility Vocabulary." ;
        rdfs:isDefinedBy               mv: ;
        rdfs:label                     "MobiVoc: Open Mobility Vocabulary"@en ;
        cc:license                     <http://creativecommons.org/licenses/by/4.0/> ;
        dct:contributor                <http://purl.org/net/clange> ;
        dct:creator                    ecc:aweilandt , ecc:mbruemmer ;
        dct:modified                   "2017-05-15"^^xsd:date ;
        dct:publisher                  ecc:eccenca-GmbH ;
        vann:preferredNamespacePrefix  "mv" ;
        vann:preferredNamespaceUri     "http://schema.mobivoc.org/" ;
        void:vocabulary                vann: , foaf: ;
        owl:versionInfo                "1.0.0" .

mv:ParkingUsageType  a    owl:Class , rdfs:Class ;
        rdfs:comment      "A type of special purpose a parking space is designated for, like women's parking spaces."@en ;
        rdfs:isDefinedBy  mv: ;
        rdfs:label        "Parking usage type"@en , "Stellplatz Nutzungsart"@de ;
        owl:deprecated    true ;
        skos:note         "Deprecated, use validForUserGroup [a UserGroup] instead." .

vann:preferredNamespacePrefix
        a                 owl:AnnotationProperty ;
        rdfs:isDefinedBy  vann: .

mv:isFastChargeCapable
        a                 owl:DatatypeProperty , rdf:Property ;
        rdfs:comment      "Indicates that the charger is able to fast charge." ;
        rdfs:domain       mv:Charger ;
        rdfs:isDefinedBy  mv: ;
        rdfs:label        "is fast charge capable"@en , "erlaubt Schnellladen"@de ;
        rdfs:range        xsd:boolean .

ecc:mbruemmer  a   foaf:Person , dct:Agent ;
        foaf:name  "Martin Brümmer" .

mv:timeStartValue  a      owl:DatatypeProperty , rdf:Property ;
        rdfs:comment      "Indicates the start value of a time period." ;
        rdfs:domain       mv:TimeSpecification ;
        rdfs:isDefinedBy  mv: ;
        rdfs:label        "Anfangszeit"@de , "time start value"@en ;
        rdfs:range        xsd:float .

mv:powerInKW  a           owl:DatatypeProperty , rdf:Property ;
        rdfs:comment      "Indicates the power of a charger or plug in kilowatts." ;
        rdfs:domain       [ a            owl:Class ;
                            owl:unionOf  ( mv:Plug mv:Charger )
                          ] ;
        rdfs:isDefinedBy  mv: ;
        rdfs:label        "power in kW"@en ;
        rdfs:range        xsd:double .

mv:CarsharingUsers  a     mv:UserGroup ;
        rdfs:comment      "User of a car rental model where people rent cars for short periods of time."@en ;
        rdfs:isDefinedBy  mv: ;
        rdfs:label        "Carsharing users"@en-us , "Car club users"@en-uk , "Carsharing-Nutzer"@de , "Utilisateurs de l'autopartage"@fr ;
        skos:hiddenLabel  "Car-sharing users" , "Car sharing users" ;
        skos:prefLabel    "Carsharing users"@en-us , "Carsharing-Nutzer"@de .

mv:voltageInV  a          owl:DatatypeProperty , rdf:Property ;
        rdfs:comment      "Indicates the voltage of a charger or plug in volt." ;
        rdfs:domain       [ a            owl:Class ;
                            owl:unionOf  ( mv:Plug mv:Charger )
                          ] ;
        rdfs:isDefinedBy  mv: ;
        rdfs:label        "voltage in V"@en ;
        rdfs:range        xsd:double .

mv:model  a               owl:DatatypeProperty , rdf:Property ;
        rdfs:comment      "Indicates the charger model of the charging point." ;
        rdfs:domain       mv:Charger ;
        rdfs:isDefinedBy  mv: ;
        rdfs:label        "model"@en , "Modell"@de ;
        rdfs:range        xsd:string .

mv:NormalParkingRestrictionsLifted
        a                 mv:CivicStructureStatus ;
        rdfs:comment      "The parking restrictions that normally apply in the specified location have been temporarily lifted." ;
        rdfs:isDefinedBy  mv: ;
        rdfs:label        "Normale Parkbeschränkungen aufgehoben"@de , "Normal parking restrictions lifted"@en .

<http://creativecommons.org/licenses/by/4.0/>
        rdfs:label  "Creative Commons Attribution 4.0 International" .

mv:SpecialParkingRestrictionsInForce
        a                 mv:CivicStructureStatus ;
        rdfs:comment      "Parking restrictions, other than those that normally apply, are in force in a specified area." ;
        rdfs:isDefinedBy  mv: ;
        rdfs:label        "Special parking restrictions in force"@en , "Besondere Parkbeschränkungen in Kraft"@de .

mv:PerpendicularParking
        a                 mv:ArrangementPattern ;
        rdfs:comment      "Bei der Senkrechtaufstellung wird das Fahrzeug mit einem Aufstellwinkel von von 100 gon (90°) geparkt."@de , "With perpendicular parking, vehicles are parked side to side, perpendicular to an aisle, curb, or wall. This type of parking is commonly used in parking lots and parking facilities."@en ;
        rdfs:isDefinedBy  mv: ;
        rdfs:label        "Senkrechtaufstellung"@de , "Perpendicular parking"@en ;
        skos:altLabel     "Bay parking"@en ;
        skos:prefLabel    "Perpendicular parking"@en .

mv:Bicycle  a             s:Vehicle ;
        rdfs:comment      "A human-or electric powered, pedal-driven, single-track vehicle, having two wheels attached to a frame, one behind the other."@en ;
        rdfs:isDefinedBy  mv: ;
        rdfs:label        "Vélo"@fr , "Fahrrad"@de , "Bicycle"@en .

mv:numberOfParkingSpacesForDisabledPersons
        a                 owl:DatatypeProperty , rdf:Property ;
        rdfs:comment      "Indicates the number of parking spaces for disabled persons." ;
        rdfs:domain       mv:ParkingFacility ;
        rdfs:isDefinedBy  mv: ;
        rdfs:label        "Anzahl Behindertenparkplätze"@de , "number of parking spaces for disabled persons"@en ;
        rdfs:range        xsd:integer ;
        owl:deprecated    true ;
        skos:note         "Deprecated, use value of Capacity resource instead." .

mv:Plug  a                owl:Class , rdfs:Class ;
        rdfs:comment      "Component of a charger to connect an electric vehicle. There are different plug types used for charging electric vehicles." ;
        rdfs:isDefinedBy  mv: ;
        rdfs:label        "Plug"@en , "Anschluss"@de .

mv:chargerQuantity  a     owl:DatatypeProperty , rdf:Property ;
        rdfs:comment      "Indicates the amount of chargers available at the charging point." ;
        rdfs:domain       mv:Charger ;
        rdfs:isDefinedBy  mv: ;
        rdfs:label        "charger quantity"@en , "Anzahl Ladepunkte"@de ;
        rdfs:range        xsd:integer .

mv:SEV1011_Type_J  a        mv:PlugType ;
        rdfs:comment        "The Swiss standard, also used in Liechtenstein, is SN SEV 1011:2009 Plugs and socket-outlets for household and similar purposes. The standard defines a hierarchical system of plugs and sockets with two, three and five pins, and 10 A or 16 A ratings. Sockets will accept plugs with the same or fewer pins and the same or lower ratings." ;
        rdfs:isDefinedBy    mv: ;
        rdfs:label          "SEV1011 Type J"@en ;
        rdfs:seeAlso        <https://en.wikipedia.org/wiki/AC_power_plugs_and_sockets#10_A_plugs_and_sockets_(Type_J)> ;
        mv:ocmConnectionID  "1037" ;
        skos:altLabel       "Type J" , "Swiss domestic 3-pin" ;
        foaf:depiction      <https://upload.wikimedia.org/wikipedia/commons/d/da/AC_Power_Plug_Type_J.jpg> .

mv:totalCapacity  a       owl:DatatypeProperty , rdf:Property ;
        rdfs:comment      "Indicates the total number of parking spaces of a parking facility." ;
        rdfs:domain       mv:ParkingFacility ;
        rdfs:isDefinedBy  mv: ;
        rdfs:label        "Gesamtkapazität"@de , "total capacity"@en ;
        rdfs:range        xsd:integer .

mv:queuingTime  a         owl:DatatypeProperty , rdf:Property ;
        rdfs:comment      "The current queuing time (duration) for entering the parking facility." ;
        rdfs:domain       mv:ParkingFacility ;
        rdfs:isDefinedBy  mv: ;
        rdfs:label        "Wartezeit"@de , "queuing time"@en ;
        rdfs:range        xsd:string .

mv:ParkingLot  a          rdfs:Class , owl:Class ;
        rdfs:comment      "Parking area on a single groundfloor level that is usually located outdoor." ;
        rdfs:isDefinedBy  mv: ;
        rdfs:label        "Parking lot"@en , "Parkplatz"@de ;
        rdfs:subClassOf   mv:ParkingFacility ;
        skos:altLabel     "car lot"@en , "Parkfläche"@de ;
        skos:prefLabel    "Parking lot"@en-us , "Parkplatz"@de , "Car park"@en-uk .

mv:SAE_J1772-2001  a        mv:PlugType ;
        rdfs:comment        "SAE J1772 (IEC Type 1) is a North American standard for electrical connectors for electric vehicles maintained by the SAE International and has the formal title \"SAE Surface Vehicle Recommended Practice J1772, SAE Electric Vehicle Conductive Charge Coupler\"." ;
        rdfs:isDefinedBy    mv: ;
        rdfs:label          "J1772"@en ;
        rdfs:seeAlso        <https://en.wikipedia.org/wiki/SAE_J1772> ;
        mv:ocmConnectionID  "7" .

vann:preferredNamespaceUri
        a                 owl:AnnotationProperty ;
        rdfs:isDefinedBy  vann: .

mv:Mennekes_Type_2  a       mv:PlugType ;
        rdfs:comment        "The IEC 62196 Type 2 connector (commonly referred to as Mennekes) is used for charging electric cars within Europe. The connector is circular in shape, with a flattened top edge and originally specified for charging battery electric vehicles at 3–120 kilowatts." ;
        rdfs:isDefinedBy    mv: ;
        rdfs:label          "Mennekes (Type 2)"@en ;
        rdfs:seeAlso        <https://en.wikipedia.org/wiki/Type_2_connector> ;
        mv:ocmConnectionID  "25" , "1036" ;
        skos:altLabel       "IEC_62196 Type 2" ;
        foaf:depiction      <https://upload.wikimedia.org/wikipedia/commons/f/f3/VDE-AR-E_2623-2-2-plug.jpg> .

mv:CEE_7_5  a               mv:PlugType ;
        rdfs:comment        "The CEE 7/5 socket and CEE 7/6 plug are defined in French standard NF C 61-314 \"Plugs and socket-outlets for household and similar purposes\" (which also includes CEE 7/7, 7/16 and 7/17 plugs) The socket has a predominantly circular recess which is 15 mm (0.591 in) deep with two symmetrical round apertures and a round 4.8 mm (0.189 in) earth pin projecting from the socket such that the tip is 23 mm (0.906 in) beyond the live contacts, to ensure that the earth is always engaged before live pin contact is made. The earth pin is centred between the apertures, offset by 10 mm (0.394 in). The plug (which is often, in error, also referred to as CEE 7/5) has two round pins measuring 4.8 by 19 mm (0.189 by 0.748 in), spaced 19 mm (0.748 in) apart and with an aperture for the socket's projecting earth pin. This standard is also used in Belgium, Poland, the Czech Republic, Slovakia and some other countries." ;
        rdfs:isDefinedBy    mv: ;
        rdfs:label          "CEE 7/5"@en ;
        rdfs:seeAlso        <https://en.wikipedia.org/wiki/AC_power_plugs_and_sockets#CEE_7/5_socket_and_CEE_7/6_plug_(French;_Type_E)> ;
        mv:ocmConnectionID  "23" ;
        skos:altLabel       "Type E" ;
        foaf:depiction      <https://upload.wikimedia.org/wikipedia/commons/thumb/b/b3/E_plug_and_socket.jpg/1920px-E_plug_and_socket.jpg> .

dct:date  a               owl:DatatypeProperty , rdf:Property ;
        rdfs:comment      "The date of the given real-time capacity."@en ;
        rdfs:domain       mv:RealTimeCapacity ;
        rdfs:isDefinedBy  dct: ;
        rdfs:label        "date"@en ;
        rdfs:range        xsd:datetime .

mv:IEC_60309_5-pin  a       mv:PlugType ;
        rdfs:comment        "IEC 60309 (formerly IEC 309 and CEE 17, also published by CENELEC as EN 60309) is an international standard from the International Electrotechnical Commission (IEC) for \"plugs, socket-outlets and couplers for industrial purposes\". 5-Pin connector." ;
        rdfs:isDefinedBy    mv: ;
        rdfs:label          "IEC_60309 5-pin"@en ;
        rdfs:seeAlso        <https://en.wikipedia.org/wiki/IEC_60309> ;
        mv:ocmConnectionID  "17" ;
        foaf:depiction      <https://upload.wikimedia.org/wikipedia/commons/thumb/2/2a/CEE-Stecker.jpg/1280px-CEE-Stecker.jpg> .

mv:name  a                owl:DatatypeProperty , rdf:Property ;
        rdfs:comment      "Name of the civic structure or facility." ;
        rdfs:domain       s:CivicStructure ;
        rdfs:isDefinedBy  mv: ;
        rdfs:label        "name"@en , "Name"@de ;
        rdfs:range        xsd:string .

mv:TaxiParkingSpace  a    mv:ParkingUsageType ;
        rdfs:comment      "Parking space where only taxis are allowed to."@en ;
        rdfs:isDefinedBy  mv: ;
        rdfs:label        "Taxi parking space"@en , "Taxi-Stellplatz"@de ;
        owl:deprecated    true ;
        skos:note         "Deprecated, use validForUserGroup [a UserGroup] instead." .

mv:NEMA_14-50  a            mv:PlugType ;
        rdfs:comment        "NEMA connectors are power plugs and receptacles used for AC mains electricity in North America and other countries that use the standards set by the US National Electrical Manufacturers Association. The NEMA 14 devices are four-wire grounding devices (hot-hot-neutral-ground) available in ratings from 15 to 60 A. The voltage rating is 250 V. Rated for 60A." ;
        rdfs:isDefinedBy    mv: ;
        rdfs:label          "NEMA 14-50"@en ;
        rdfs:seeAlso        <https://en.wikipedia.org/wiki/NEMA_connector#NEMA_14> ;
        mv:ocmConnectionID  "11" ;
        foaf:depiction      <https://upload.wikimedia.org/wikipedia/commons/d/d3/220sb.svg> .

mv:Action  a              owl:Class ;
        rdfs:comment      "Action that is done."@en ;
        rdfs:isDefinedBy  mv: ;
        rdfs:label        "Aktion"@de , "Action"@en .

mv:AutomatedParkingGarage
        a                 owl:Class , rdfs:Class ;
        rdfs:comment      "Parking garage with an automated parking system that automatically moves cars to the available parking space somewhere in the garage."@en ;
        rdfs:isDefinedBy  mv: ;
        rdfs:label        "Automatisches Parkhaus"@de , "Automated parking garage"@en ;
        rdfs:subClassOf   mv:ParkingFacility .

mv:CEE_7-Pin  a             mv:PlugType ;
        rdfs:comment        "CEE 7-Pin 32A / 400V Socket." ;
        rdfs:isDefinedBy    mv: ;
        rdfs:label          "CEE 7-Pin"@en ;
        mv:ocmConnectionID  "18" .

mv:ParkingFacilityExit
        a                 owl:Class , rdfs:Class ;
        rdfs:comment      "Exit of a parking facility where vehicles can leave the parking facility."@en ;
        rdfs:isDefinedBy  mv: ;
        rdfs:label        "Exit"@en , "Ausfahrt"@de ;
        rdfs:subClassOf   s:CivicStructure .

mv:SAE_J1772-2009  a        mv:PlugType ;
        rdfs:comment        "SAE J1772 (IEC Type 1) is a North American standard for electrical connectors for electric vehicles maintained by the SAE International and has the formal title \"SAE Surface Vehicle Recommended Practice J1772, SAE Electric Vehicle Conductive Charge Coupler\". \n    The SAE J1772-2009 connector specification has been added to the international IEC 62196-2 standard." ;
        rdfs:isDefinedBy    mv: ;
        rdfs:label          "J1772 2009"@en ;
        rdfs:seeAlso        <https://en.wikipedia.org/wiki/IEC_62196#Type_1_(SAE_J1772-2009),_Yazaki> ;
        mv:ocmConnectionID  "1" ;
        skos:altLabel       "IEC 62196 Type 1" ;
        foaf:depiction      <https://upload.wikimedia.org/wikipedia/commons/thumb/e/e0/SAE_J1772_7058855567.jpg/1280px-SAE_J1772_7058855567.jpg> .

s:openingHoursSpecification
        a                 owl:ObjectProperty , rdf:Property ;
        rdfs:comment      "Indicates the general opening hours for a business or civic structure."@en ;
        rdfs:domain       s:CivicStructure ;
        rdfs:isDefinedBy  s: ;
        rdfs:label        "opening hours specification"@en ;
        rdfs:range        s:OpeningHoursSpecification .

mv:BikeAndRide  a         mv:ParkingFacilityConnection ;
        rdfs:comment      "Parking facilities for bicycles with connection to public transport." ;
        rdfs:isDefinedBy  mv: ;
        rdfs:label        "Bike and Ride" .

mv:ParkingFacility  a        owl:Class , rdfs:Class ;
        rdfs:comment         "Any facility or area assigned for parking vehicles. A parking facility can provide one or more parking spaces."@en ;
        rdfs:isDefinedBy     mv: ;
        rdfs:label           "Parking facility"@en , "Parkeinrichtung"@de ;
        rdfs:subClassOf      s:CivicStructure ;
        owl:equivalentClass  s:ParkingFacility .

s:acceptedPaymentMethod
        a                 owl:ObjectProperty ;
        rdfs:comment      "The payment method(s) accepted by seller for this offer."@en ;
        rdfs:domain       s:CivicStructure ;
        rdfs:isDefinedBy  s: ;
        rdfs:label        "accepted payment method"@en ;
        rdfs:range        s:PaymentMethod .

mv:Tesla_Supercharger
        a                   mv:PlugType ;
        rdfs:comment        "The Tesla Supercharger network is a system of 480-volt DC fast-charging stations built by American vehicle manufacturer Tesla Inc. to allow longer journeys for their all-electric manufactured vehicles (Model S, 3 and X), through quick charging of the vehicle's battery packs." ;
        rdfs:isDefinedBy    mv: ;
        rdfs:label          "Tesla Supercharger"@en ;
        rdfs:seeAlso        <https://en.wikipedia.org/wiki/Tesla_Supercharger> ;
        mv:ocmConnectionID  "30" , "27" ;
        foaf:depiction      <https://upload.wikimedia.org/wikipedia/commons/thumb/4/49/Tesla-type-2-model-s-charge-port-inlet-0996.jpg/1280px-Tesla-type-2-model-s-charge-port-inlet-0996.jpg> .

mv:ParkAndRideServiceNotOperating
        a                 mv:CivicStructureStatus ;
        rdfs:comment      "Park and ride services are not operating until the specified time." ;
        rdfs:isDefinedBy  mv: ;
        rdfs:label        "Park and ride service not operating"@en , "Kein P+R-Service"@de .

mv:timeUnit  a            owl:DatatypeProperty , rdf:Property ;
        rdfs:comment      "Indicates the time unit a value is specified for." ;
        rdfs:domain       mv:TimeSpecification ;
        rdfs:isDefinedBy  mv: ;
        rdfs:label        "Zeiteinheit"@de , "time unit"@en ;
        rdfs:range        xsd:string .

mv:WomensParkingSpace
        a                 mv:ParkingUsageType ;
        rdfs:comment      "Specially designated and identified parking space to be used by women."@en , "Gekennzeichneter und ausgewiesener Stellplatz für die Nutzung durch Frauen."@de ;
        rdfs:isDefinedBy  mv: ;
        rdfs:label        "Frauenparkplatz"@de , "Women's parking space"@en ;
        owl:deprecated    true ;
        skos:altLabel     "Damenparkplatz"@de-at , "Ladies' parking space"@en ;
        skos:note         "Deprecated, use validForUserGroup [a UserGroup] instead." ;
        skos:prefLabel    "Women's parking space"@en .

mv:CarsharingParkingSpace
        a                 mv:ParkingUsageType ;
        rdfs:comment      "Specially designated and identified parking space reserved for carsharing vehicles."@en ;
        rdfs:isDefinedBy  mv: ;
        rdfs:label        "Place de stationnement pour l'autopartage"@fr , "Carsharing parking space"@en , "Carsharing-Stellplatz"@de ;
        owl:deprecated    true ;
        skos:note         "Deprecated, use validForUserGroup [a UserGroup] instead." .

s:PriceSpecification  a   owl:Class ;
        rdfs:comment      "A structured value representing a price or price range for an item."@en ;
        rdfs:isDefinedBy  s: ;
        rdfs:label        "Preisspezifikation"@de , "Price specification"@en .

mv:numberOfCarsharingParkingSpaces
        a                 rdf:Property , owl:DatatypeProperty ;
        rdfs:comment      "Indicates the number of parking spaces that are reserved for carsharing." ;
        rdfs:domain       mv:ParkingFacility ;
        rdfs:isDefinedBy  mv: ;
        rdfs:label        "number of carsharing spaces"@en , "Anzahl Carsharing-Parkplätze"@de ;
        rdfs:range        xsd:integer ;
        owl:deprecated    true ;
        skos:note         "Deprecated, use value of Capacity resource instead." .

mv:CivicStructureStatus
        a                 owl:Class , rdfs:Class ;
        rdfs:comment      "Status information of a civic structure." ;
        rdfs:isDefinedBy  mv: ;
        rdfs:label        "Status der Parkeinrichtung"@de , "Civic structure status"@en .

mv:exit  a                owl:ObjectProperty , rdf:Property ;
        rdfs:comment      "Describes the exit of a parking facility." ;
        rdfs:domain       mv:ParkingFacility ;
        rdfs:isDefinedBy  mv: ;
        rdfs:label        "hat Ausfahrt"@de , "exit"@en ;
        rdfs:range        mv:ParkingFacilityExit .

mv:ParkAndFly  a          mv:ParkingFacilityConnection ;
        rdfs:comment      "Connection to airport." ;
        rdfs:isDefinedBy  mv: ;
        rdfs:label        "Parken und Fliegen"@de , "Park & Fly" ;
        skos:altLabel     "P+F" , "P&F" .

mv:TaxiDrivers  a         mv:UserGroup ;
        rdfs:comment      "Drivers of a vehicle for hire, used by a single passenger or small group of passengers, often for a non-shared ride. Taxi drivers convey passengers between locations of their choice."@en ;
        rdfs:isDefinedBy  mv: ;
        rdfs:label        "Taxifahrer"@de , "Taxi drivers"@en ;
        skos:altLabel     "Taxicab drivers"@en , "Cabbies"@en-uk , "Cab drivers"@en ;
        skos:prefLabel    "Taxi drivers"@en , "Taxifahrer"@de .

mv:NEMA_6-20  a             mv:PlugType ;
        rdfs:comment        "NEMA connectors are power plugs and receptacles used for AC mains electricity in North America and other countries that use the standards set by the US National Electrical Manufacturers Association.\nAll NEMA 6 devices are three-wire grounding devices (hot-hot-ground) used for 208 and 240 V circuits and rated for 250 V maximum. The 20 A plug has a blade rotated 90°." ;
        rdfs:isDefinedBy    mv: ;
        rdfs:label          "NEMA 6-20"@en ;
        rdfs:seeAlso        <https://en.wikipedia.org/wiki/NEMA_connector#NEMA_6> ;
        mv:ocmConnectionID  "14" ;
        foaf:depiction      <https://upload.wikimedia.org/wikipedia/commons/thumb/0/0d/NEMA_simplified_pins.svg/765px-NEMA_simplified_pins.svg.png> .

mv:BusOrCoach  a          s:Vehicle ;
        rdfs:comment      "A bus is a road vehicle designed to carry passengers. Coaches are luxury busses, usually in service for long distance travel."@en ;
        rdfs:isDefinedBy  mv: ;
        rdfs:label        "Bus"@de , "Coach"@en .

mv:ParkingFacilityConnection
        a                 owl:Class , rdfs:Class ;
        rdfs:comment      "Transport connections available at the parking facility (e.g. Park & Ride)." ;
        rdfs:isDefinedBy  mv: ;
        rdfs:label        "Parking facility connections"@en , "Anschlussmöglichkeiten der Parkeinrichtung"@de .

mv:VideoSurveillance  a   mv:ParkingFacilityFeature ;
        rdfs:comment      "The parking facility is surveilled by video."@en ;
        rdfs:isDefinedBy  mv: ;
        rdfs:label        "Videoüberwachung"@de , "Video surveillance"@en .

mv:currentInA  a          owl:DatatypeProperty , rdf:Property ;
        rdfs:comment      "Indicates the current of a charger or plug in ampere." ;
        rdfs:domain       [ a            owl:Class ;
                            owl:unionOf  ( mv:Plug mv:Charger )
                          ] ;
        rdfs:isDefinedBy  mv: ;
        rdfs:label        "current in A"@en ;
        rdfs:range        xsd:double .

mv:numberOfOccupiedParkingSpaces
        a                 owl:DatatypeProperty , rdf:Property ;
        rdfs:comment      "Indicates the number of currently occupied parking spaces." ;
        rdfs:domain       mv:ParkingFacility ;
        rdfs:isDefinedBy  mv: ;
        rdfs:label        "number of occupied parking spaces"@en , "Anzahl belegter Stellplätze"@de ;
        rdfs:range        xsd:integer ;
        owl:deprecated    true ;
        skos:note         "Deprecated, use value of Capacity resource instead." .

mv:ocmConnectionID  a     owl:AnnotationProperty ;
        rdfs:comment      "The OpenChargeMap ID used for the Connection / Plug." ;
        rdfs:isDefinedBy  mv: ;
        rdfs:label        "ocm connection ID"@en ;
        rdfs:range        xsd:string .

geo:lat  a                owl:DatatypeProperty , rdf:Property ;
        rdfs:comment      "Geographic latitude of a place."@en ;
        rdfs:domain       s:Place ;
        rdfs:isDefinedBy  geo: ;
        rdfs:label        "latitude"@en ;
        rdfs:range        xsd:string .

mv:Families  a            mv:UserGroup ;
        rdfs:comment      "Parents with children."@en ;
        rdfs:isDefinedBy  mv: ;
        rdfs:label        "Familien"@de , "Families"@en .

mv:NEMA_5-20R  a            mv:PlugType ;
        rdfs:comment        "NEMA connectors are power plugs and receptacles used for AC mains electricity in North America and other countries that use the standards set by the US National Electrical Manufacturers Association. All NEMA 5 devices are three-wire grounding devices (hot-neutral-ground) rated for 125 V maximum." ;
        rdfs:isDefinedBy    mv: ;
        rdfs:label          "NEMA 5-20R"@en ;
        rdfs:seeAlso        <https://en.wikipedia.org/wiki/NEMA_connector#NEMA_5> ;
        mv:ocmConnectionID  "9" ;
        foaf:depiction      <https://upload.wikimedia.org/wikipedia/commons/thumb/4/42/Electrical_outlet_with_label.jpg/1280px-Electrical_outlet_with_label.jpg> .

mv:vehicleHeightLimitInM
        a                 owl:DatatypeProperty , rdf:Property ;
        rdfs:comment      "Indicates the height limit in meter for vehicles using the parking facility." ;
        rdfs:domain       s:CivicStructure ;
        rdfs:isDefinedBy  mv: ;
        rdfs:label        "Höhenbegrenzung für Fahrzeuge"@de , "vechicle height limit"@en ;
        rdfs:range        xsd:decimal .

mv:BicycleParkingStation
        a                 owl:Class , rdfs:Class ;
        rdfs:comment      "Building or structure designed for use as a bicycle parking facility."@en ;
        rdfs:isDefinedBy  mv: ;
        rdfs:label        "Fahrradparkstation"@de , "Bicycle parking station"@en ;
        rdfs:subClassOf   mv:ParkingFacility .

mv:Motorbike  a           s:Vehicle ;
        rdfs:comment      "A single-track, two-wheeled motor vehicle."@en ;
        rdfs:isDefinedBy  mv: ;
        rdfs:label        "Motorrad"@de , "Motorbike"@en ;
        skos:altLabel     "Motorcycle"@en ;
        skos:prefLabel    "Moto"@fr , "Motorrad"@de , "Motorbike"@en .

mv:Car  a                 s:Vehicle ;
        rdfs:comment      "A wheeled, self-powered motor vehicle used for transportation."@en ;
        rdfs:isDefinedBy  mv: ;
        rdfs:label        "Voiture"@fr , "Car"@en , "Auto"@de ;
        skos:altLabel     "Pkw"@de .

mv:NEMA_5-15R  a            mv:PlugType ;
        rdfs:comment        "NEMA connectors are power plugs and receptacles used for AC mains electricity in North America and other countries that use the standards set by the US National Electrical Manufacturers Association. All NEMA 5 devices are three-wire grounding devices (hot-neutral-ground) rated for 125 V maximum.\n   The 5-15R is by far the most common electrical receptacle in North America in buildings built since the mid-twentieth century. It is usually installed in a duplex configuration; two receptacles may share a common circuit or may each be wired separately, sometimes to a switch." ;
        rdfs:isDefinedBy    mv: ;
        rdfs:label          "NEMA 5-15R"@en ;
        rdfs:seeAlso        <https://en.wikipedia.org/wiki/NEMA_connector#NEMA_5> ;
        mv:ocmConnectionID  "22" ;
        foaf:depiction      <https://upload.wikimedia.org/wikipedia/commons/thumb/0/0d/NEMA_simplified_pins.svg/765px-NEMA_simplified_pins.svg.png> .

mv:parkingSpace  a        owl:ObjectProperty , rdf:Property ;
        rdfs:comment      "Relates the parking facility to a contained parking space."@en ;
        rdfs:domain       mv:ParkingFacility ;
        rdfs:isDefinedBy  mv: ;
        rdfs:label        "hat Stellplatz"@de , "parking space"@en ;
        rdfs:range        mv:ParkingSpace .

mv:ParkingFacilityFeature
        a                 owl:Class , rdfs:Class ;
        rdfs:comment      "Features of the parking facility (e.g. parking for disabled people)." ;
        rdfs:isDefinedBy  mv: ;
        rdfs:label        "Parking facility feature"@en , "Ausstattung der Parkeinrichtung"@de .

mv:Truck  a               s:Vehicle ;
        rdfs:comment      "A motor vehicle designed to transport cargo."@en ;
        rdfs:isDefinedBy  mv: ;
        rdfs:label        "Lkw"@de , "Truck"@en .

mv:capacity  a            owl:ObjectProperty , rdf:Property ;
        rdfs:comment      "Relates the civic structure to its capacity."@en ;
        rdfs:domain       s:CivicStructure ;
        rdfs:isDefinedBy  mv: ;
        rdfs:label        "hat Kapazität"@de , "has capacity"@en ;
        rdfs:range        mv:Capacity .

mv:validForVehicle  a     owl:ObjectProperty , rdf:Property ;
        rdfs:comment      "Indicates that an entity is valid for a specific type of vehicle."@en ;
        rdfs:domain       [ a            owl:Class ;
                            owl:unionOf  ( mv:AccessCondition s:PriceSpecification mv:Capacity )
                          ] ;
        rdfs:isDefinedBy  mv: ;
        rdfs:label        "gültig für Fahrzeug"@de , "valid for vehicle"@en ;
        rdfs:range        s:Vehicle .

mv:Restrict  a            mv:Action ;
        rdfs:comment      "An action is restricted."@en ;
        rdfs:isDefinedBy  mv: ;
        rdfs:label        "Beschränken"@de , "Restrict"@en .

mv:Charger  a             owl:Class , rdfs:Class ;
        rdfs:comment      "Component of a charging point used to charge electric vehicles. A charging point can have one or more chargers." ;
        rdfs:isDefinedBy  mv: ;
        rdfs:label        "Ladegerät"@de , "Charger"@en .

mv:additionalInformation
        a                 owl:DatatypeProperty , rdf:Property ;
        rdfs:comment      "Further information about the civic structure or facility."@en ;
        rdfs:domain       s:CivicStructure ;
        rdfs:isDefinedBy  mv: ;
        rdfs:label        "zusätzliche Information"@de , "additional information"@en ;
        rdfs:range        xsd:string .

mv:NEMA_6-15  a             mv:PlugType ;
        rdfs:comment        "NEMA connectors are power plugs and receptacles used for AC mains electricity in North America and other countries that use the standards set by the US National Electrical Manufacturers Association.\nAll NEMA 6 devices are three-wire grounding devices (hot-hot-ground) used for 208 and 240 V circuits and rated for 250 V maximum. The 6-15 resembles the 5-15, but with collinear horizontal pins" ;
        rdfs:isDefinedBy    mv: ;
        rdfs:label          "NEMA 6-15"@en ;
        rdfs:seeAlso        <https://en.wikipedia.org/wiki/NEMA_connector#NEMA_6> ;
        mv:ocmConnectionID  "15" ;
        foaf:depiction      <https://upload.wikimedia.org/wikipedia/commons/thumb/8/86/Nema_6-15.svg/346px-Nema_6-15.svg.png> .

mv:ownedBy  a             owl:ObjectProperty , rdf:Property ;
        rdfs:comment      "The owner of a civic structure or facility. Owner and operator can be different business entities."@en ;
        rdfs:domain       s:CivicStructure ;
        rdfs:isDefinedBy  mv: ;
        rdfs:label        "in Besitz von"@de , "owned by"@en ;
        rdfs:range        gr:BusinessEntity .

mv:id   a                 owl:DatatypeProperty , rdf:Property ;
        rdfs:comment      "ID of the entity." ;
        rdfs:isDefinedBy  mv: ;
        rdfs:label        "ID"@en , "ID"@de ;
        rdfs:range        xsd:string .

dct:modified  a           owl:AnnotationProperty ;
        rdfs:isDefinedBy  dct: .

mv:ParkAndRail  a         mv:ParkingFacilityConnection ;
        rdfs:comment      "Connection to railway station." ;
        rdfs:isDefinedBy  mv: ;
        rdfs:label        "Park and Rail" .

mv:PayStation  a          mv:ParkingFacilityFeature ;
        rdfs:comment      "The parking facility has a pay station."@en ;
        rdfs:isDefinedBy  mv: ;
        rdfs:label        "Pay station"@en , "Kassenautomat"@de .

dct:rights  a             owl:AnnotationProperty ;
        rdfs:isDefinedBy  dct: .

mv:OnlyAFewParkingSpacesAvailable
        a                 mv:CivicStructureStatus ;
        rdfs:comment      "The parking facility has 95% or greater occupancy." ;
        rdfs:isDefinedBy  mv: ;
        rdfs:label        "Only a few parking spaces available"@en , "Nur noch wenige Stellplätze frei"@de .

mv:numberOfMotorbikeParkingSpaces
        a                 owl:DatatypeProperty , rdf:Property ;
        rdfs:comment      "Indicates the number of parking spaces for motorbikes." ;
        rdfs:domain       mv:ParkingFacility ;
        rdfs:isDefinedBy  mv: ;
        rdfs:label        "number of parking spaces for motorbikes"@en , "Anzahl Motorradparkplätze"@de ;
        rdfs:range        xsd:integer ;
        owl:deprecated    true ;
        skos:note         "Deprecated, use value of Capacity resource instead." .

mv:NoParkingInformationAvailable
        a                 mv:CivicStructureStatus ;
        rdfs:comment      "Parking information is not available until a specified time." ;
        rdfs:isDefinedBy  mv: ;
        rdfs:label        "No parking information available"@en , "Keine Parkinformationen verfügbar"@de .

<http://purl.org/net/clange>
        a              dct:Agent ;
        foaf:homepage  <http://langec.wordpress.com/about/> ;
        foaf:name      "Christoph Lange" .

mv:BS1363  a                mv:PlugType ;
        rdfs:comment        "13 A plugs socket-outlets adaptors and connection units is a British Standard which specifies the most common type of single-phase AC power plugs and sockets that are used in the United Kingdom." ;
        rdfs:isDefinedBy    mv: ;
        rdfs:label          "BS1363"@en ;
        rdfs:seeAlso        <https://en.wikipedia.org/wiki/AC_power_plugs_and_sockets:_British_and_related_types#International_usage_of_Type_G> ;
        mv:ocmConnectionID  "3" ;
        skos:altLabel       "Type G" ;
        foaf:depiction      <https://upload.wikimedia.org/wikipedia/commons/0/00/British_plug.jpg> .

mv:action  a              owl:ObjectProperty , rdf:Property ;
        rdfs:comment      "Indicates which action is applied."@en ;
        rdfs:domain       mv:AccessCondition ;
        rdfs:isDefinedBy  mv: ;
        rdfs:label        "action"@en ;
        rdfs:range        mv:Action .

dct:creator  a            owl:AnnotationProperty ;
        rdfs:isDefinedBy  dct: .

mv:picture  a             owl:DatatypeProperty , rdf:Property ;
        rdfs:comment      "URL of the picture of a civic structure or facility."@en ;
        rdfs:domain       s:CivicStructure ;
        rdfs:isDefinedBy  mv: ;
        rdfs:label        "Bild"@de , "picture"@en ;
        rdfs:range        xsd:string .

mv:TimeSpecification  a   owl:Class ;
        rdfs:comment      "Specific time a price specification is due for."@en ;
        rdfs:isDefinedBy  mv: ;
        rdfs:label        "Zeitspezifikation"@de , "Time specification"@en .

mv:Full  a                mv:CivicStructureStatus ;
        rdfs:comment      "The parking facility is completely occupied." ;
        rdfs:isDefinedBy  mv: ;
        rdfs:label        "Full"@en , "Belegt"@de .

mv:ParkingSpace  a        rdfs:Class , owl:Class ;
        rdfs:comment      "A parking space is a location that is designated for parking a vehicle. A parking space has a certain size, is sometimes marked and can be located at roadside or inside a parking facility. Depending on the location of the parking space, there can be regulations regarding the time allowed to park and a fee paid to use the parking space."@en ;
        rdfs:isDefinedBy  mv: ;
        rdfs:label        "Parking space"@en , "Stellplatz"@de ;
        rdfs:subClassOf   s:CivicStructure ;
        skos:hiddenLabel  "Parkplatz"@de ;
        skos:prefLabel    "Stellplatz"@de , "Parking space"@en .

mv:unspecifiedCharge  a   owl:DatatypeProperty , rdf:Property ;
        rdfs:comment      "Indicates that a charge has to be paid for the usage of the civic structure." ;
        rdfs:domain       s:PriceSpecification ;
        rdfs:isDefinedBy  mv: ;
        rdfs:label        "kostenpflichtig"@de , "unspecified charge"@en ;
        rdfs:range        xsd:boolean .

mv:currentType  a         owl:DatatypeProperty , rdf:Property ;
        rdfs:comment      "Indicates the current type (AC/DC) of the plug." ;
        rdfs:domain       [ a            owl:Class ;
                            owl:unionOf  ( mv:Plug mv:Charger )
                          ] ;
        rdfs:isDefinedBy  mv: ;
        rdfs:label        "current type"@en ;
        rdfs:range        xsd:string .

mv:XLR4  a                  mv:PlugType ;
        rdfs:comment        "The XLR connector is a style of electrical connector, primarily found on professional audio, video, and stage lighting equipment. The connectors are circular in design and have between 3 and 7 pins. They are most commonly associated with balanced audio interconnection, including AES3 digital audio, but are also used for lighting control, low-voltage power supplies, and other applications. XLR connectors are available from a number of manufacturers and are covered by an international standard for dimensions, IEC 61076-2-103.[1] They are superficially similar to the older and smaller DIN connector range, but are not physically compatible with them." ;
        rdfs:isDefinedBy    mv: ;
        rdfs:label          "XLR 4-Pin"@en ;
        rdfs:seeAlso        <https://en.wikipedia.org/wiki/XLR_connector#Four-pin_(XLR4)> ;
        mv:ocmConnectionID  "21" .

mv:StatusUnknown  a       mv:CivicStructureStatus ;
        rdfs:comment      "The status of the parking facility is unknown." ;
        rdfs:isDefinedBy  mv: ;
        rdfs:label        "Status unknown"@en , "Status unbekannt"@de .

mv:EnoughParkingSpacesAvailable
        a                 mv:CivicStructureStatus ;
        rdfs:comment      "The parking facility has parking spaces available." ;
        rdfs:isDefinedBy  mv: ;
        rdfs:label        "Genügend Stellplätze frei"@de , "Enough parking spaces available"@en .

mv:SurveillanceBySecurityGuards
        a                 mv:ParkingFacilityFeature ;
        rdfs:comment      "The parking facility is surveilled by security guards."@en ;
        rdfs:isDefinedBy  mv: ;
        rdfs:label        "surveillance by security guards"@en , "Bewacht durch Personal"@de .

mv:ParkingFacilityEntrance
        a                 owl:Class , rdfs:Class ;
        rdfs:comment      "Entrance of a parking facility where vehicles can enter the parking facility."@en ;
        rdfs:isDefinedBy  mv: ;
        rdfs:label        "Entrance"@en , "Einfahrt"@de ;
        rdfs:subClassOf   s:CivicStructure .

mv:RealTimeCapacity  a    owl:Class , rdfs:Class ;
        rdfs:comment      "Real-time capacity of a parking facility or parking space."@en , "Real-time capacity of a civic structure."@en ;
        rdfs:isDefinedBy  mv: ;
        rdfs:label        "Real time capacity"@en , "Echtzeit Kapazität"@de ;
        rdfs:subClassOf   mv:Capacity .

s:Vehicle  a              owl:Class ;
        rdfs:comment      "A vehicle is a device that is designed or used to transport people or cargo over land, water, air, or through space."@en ;
        rdfs:isDefinedBy  s: ;
        rdfs:label        "Vehicle"@en , "Fahrzeug"@de .

mv:Inhabitants  a         mv:UserGroup ;
        rdfs:comment      "People living on the premises."@en ;
        rdfs:isDefinedBy  mv: ;
        rdfs:label        "Anwohner"@de , "Inhabitants"@en .

mv:SAE_Combo  a             mv:PlugType ;
        rdfs:comment        "The Combined Charging System is a quick charging method for battery electric vehicles delivering high-voltage direct current via a special electrical connector derived from the SAE J1772 (IEC Type 1)." ;
        rdfs:isDefinedBy    mv: ;
        rdfs:label          "SAE Combo (DC Fast Charge J1772)"@en ;
        rdfs:seeAlso        <https://en.wikipedia.org/wiki/Combined_Charging_System> ;
        mv:ocmConnectionID  "32" ;
        foaf:depiction      <https://upload.wikimedia.org/wikipedia/commons/thumb/f/fe/CCSCombo2.svg/1052px-CCSCombo2.svg.png> .

mv:numberOfLevels  a      owl:DatatypeProperty , rdf:Property ;
        rdfs:comment      "Indicates the total number of levels a parking facility has."@en ;
        rdfs:domain       mv:ParkingFacility ;
        rdfs:isDefinedBy  mv: ;
        rdfs:label        "Anzahl Ebenen"@de , "number of levels"@en ;
        rdfs:range        xsd:integer .

mv:ParkingGarage  a       owl:Class , rdfs:Class ;
        rdfs:comment      "A single level or multilevel parking building to park at." ;
        rdfs:isDefinedBy  mv: ;
        rdfs:label        "Parking garage"@en , "Parkhaus"@de ;
        rdfs:subClassOf   mv:ParkingFacility ;
        skos:altLabel     "Hochgarage"@de , "Parking structure"@en , "Car park"@en , "Parking building"@en ;
        skos:prefLabel    "Parking garage"@en , "Parkhaus"@de .

mv:rateOfOccupancy  a     owl:DatatypeProperty , rdf:Property ;
        rdfs:comment      "Indicates the percentage value of parking spaces occupied in a parking facility." ;
        rdfs:domain       mv:ParkingFacility ;
        rdfs:isDefinedBy  mv: ;
        rdfs:label        "Belegungsrate"@de , "rate of occupancy"@en ;
        rdfs:range        xsd:string .

mv:UserGroup  a           owl:Class ;
        rdfs:comment      "A group of users having a common characteristic."@en ;
        rdfs:isDefinedBy  mv: ;
        rdfs:label        "Nutzergruppe"@de , "User group"@en .

mv:timeEndValue  a        owl:DatatypeProperty , rdf:Property ;
        rdfs:comment      "Indicates the end value of a time period." ;
        rdfs:domain       mv:TimeSpecification ;
        rdfs:isDefinedBy  mv: ;
        rdfs:label        "Endzeit"@de , "time end value"@en ;
        rdfs:range        xsd:float .

mv:NEMA_14-30  a            mv:PlugType ;
        rdfs:comment        "NEMA connectors are power plugs and receptacles used for AC mains electricity in North America and other countries that use the standards set by the US National Electrical Manufacturers Association. The NEMA 14 devices are four-wire grounding devices (hot-hot-neutral-ground) available in ratings from 15 to 60 A. The voltage rating is 250 V. Rated for 30A." ;
        rdfs:isDefinedBy    mv: ;
        rdfs:label          "NEMA 14-30"@en ;
        rdfs:seeAlso        <https://en.wikipedia.org/wiki/NEMA_connector#NEMA_14> ;
        mv:ocmConnectionID  "10" ;
        foaf:depiction      <https://upload.wikimedia.org/wikipedia/commons/d/d3/220sb.svg> .

mv:fillRate  a            owl:DatatypeProperty , rdf:Property ;
        rdfs:comment      "The rate at which vehicles are entering the parking facility." ;
        rdfs:domain       mv:ParkingFacility ;
        rdfs:isDefinedBy  mv: ;
        rdfs:label        "fill rate"@en ;
        rdfs:range        xsd:string .

mv:Operational  a         mv:CivicStructureStatus ;
        rdfs:comment      "The facility is operational." ;
        rdfs:isDefinedBy  mv: ;
        rdfs:label        "Status operational"@en , "Status in Betrieb"@de .

mv:exitRate  a            owl:DatatypeProperty , rdf:Property ;
        rdfs:comment      "The rate at which vehicles are exiting the parking facility." ;
        rdfs:domain       mv:ParkingFacility ;
        rdfs:isDefinedBy  mv: ;
        rdfs:label        "exit rate"@en ;
        rdfs:range        xsd:string .

mv:CCS_Type2  a             mv:PlugType ;
        rdfs:comment        "The Combined Charging System is a quick charging method for battery electric vehicles delivering high-voltage direct current via a special electrical connector derived from the  IEC Type 2 connector. As the plug is a combination of an AC connector with a DC option the resulting connector is also called Combo Coupler and the variant with Type 2 is abbreviated as Combo2." ;
        rdfs:isDefinedBy    mv: ;
        rdfs:label          "CCS Type2"@en ;
        rdfs:seeAlso        <https://en.wikipedia.org/wiki/Combined_Charging_System> ;
        mv:ocmConnectionID  "33" ;
        skos:altLabel       "Combo2" ;
        foaf:depiction      <https://upload.wikimedia.org/wikipedia/commons/thumb/f/fe/CCSCombo2.svg/1052px-CCSCombo2.svg.png> .

mv:parkingUsageType  a    owl:ObjectProperty , rdf:Property ;
        rdfs:comment      "Relates the capacity of a parking facility to a specific designated usage type."@en ;
        rdfs:domain       mv:Capacity ;
        rdfs:isDefinedBy  mv: ;
        rdfs:label        "parking usage type"@en , "Nutzungsart"@de ;
        rdfs:range        mv:ParkingUsageType ;
        owl:deprecated    true ;
        skos:note         "Deprecated, use validForUserGroup instead." .

mv:numberOfBicycleParkingSpaces
        a                 owl:DatatypeProperty , rdf:Property ;
        rdfs:comment      "Indicates the number of parking spaces for bicycles." ;
        rdfs:domain       mv:ParkingFacility ;
        rdfs:isDefinedBy  mv: ;
        rdfs:label        "number of parking spaces for bicycles"@en , "Anzahl Fahrradparkplätze"@de ;
        rdfs:range        xsd:integer ;
        owl:deprecated    true ;
        skos:note         "Deprecated, use value of Capacity resource instead." .

mv:maximumValue  a        owl:DatatypeProperty , rdf:Property ;
        rdfs:comment      "Indicates the maximum value of the capacity."@en ;
        rdfs:domain       mv:Capacity ;
        rdfs:isDefinedBy  mv: ;
        rdfs:label        "maximum value"@en ;
        rdfs:range        xsd:integer .

mv:ArrangementPattern
        a                 owl:Class , rdfs:Class ;
        rdfs:comment      "Art und Weise, wie ein Fahrzeug auf einer Parkfläche aufgestellt wird."@de , "Pattern how parking spaces are arranged in a parking facility or at roadside."@en ;
        rdfs:isDefinedBy  mv: ;
        rdfs:label        "Aufstellart"@de , "Arrangement pattern"@en .

mv:employeeOf  a          owl:ObjectProperty , rdf:Property ;
        rdfs:comment      "Indicates that a group is employee of a specific business entity."@en ;
        rdfs:domain       mv:UserGroup ;
        rdfs:isDefinedBy  mv: ;
        rdfs:label        "Mitarbeiter von"@de , "employee of"@en ;
        rdfs:range        gr:BusinessEntity .

mv:PersonsWithDisabledParkingPermit
        a                 mv:UserGroup ;
        rdfs:comment      "Persons with disabilities having a special parking permit that gives the right to use parking spaces reserved for disabled people."@en ;
        rdfs:isDefinedBy  mv: ;
        rdfs:label        "Personen mit Behindertenparkausweis"@de , "Persons with disabled parking permit"@en .

geo:long  a               owl:DatatypeProperty , rdf:Property ;
        rdfs:comment      "Geographic longitude of a place."@en ;
        rdfs:domain       s:Place ;
        rdfs:isDefinedBy  geo: ;
        rdfs:label        "longitude"@en ;
        rdfs:range        xsd:string .

mv:AccessCondition  a     owl:Class ;
        rdfs:comment      "A condition that has to be fullfilled to get access to a civic structure."@en ;
        rdfs:isDefinedBy  mv: ;
        rdfs:label        "Zugangsbedingung"@de , "Access condition"@en .

mv:validForUserGroup  a   owl:ObjectProperty , rdf:Property ;
        rdfs:comment      "Indicates that an entity is valid for a specific group of users."@en ;
        rdfs:domain       [ a            owl:Class ;
                            owl:unionOf  ( mv:AccessCondition s:PriceSpecification mv:Capacity )
                          ] ;
        rdfs:isDefinedBy  mv: ;
        rdfs:label        "gültig für Nutzergruppe"@de , "valid for user group"@en ;
        rdfs:range        mv:UserGroup .

dct:publisher  a          owl:AnnotationProperty ;
        rdfs:isDefinedBy  dct: .

mv:CHAdeMO  a               mv:PlugType ;
        rdfs:comment        "CHAdeMO is the trade name of a quick charging method for battery electric vehicles delivering up to 62.5 kW of direct current (500 V, 125 A[1]) via a special electrical connector." ;
        rdfs:isDefinedBy    mv: ;
        rdfs:label          "CHAdeMO"@en ;
        rdfs:seeAlso        <https://en.wikipedia.org/wiki/CHAdeMO> ;
        mv:ocmConnectionID  "2" ;
        owl:sameAs          dbpedia:CHAdeMO ;
        foaf:depiction      <https://upload.wikimedia.org/wikipedia/commons/d/d3/CHAdeMO_Plug_VacavilleDavisStDC2.jpg> .

mv:energySource  a        owl:DatatypeProperty , rdf:Property ;
        rdfs:comment      "Indicates the energy source used for the charging point i.e. renewable etc." ;
        rdfs:domain       mv:ChargingPoint ;
        rdfs:isDefinedBy  mv: ;
        rdfs:label        "energy source"@en ;
        rdfs:range        xsd:string .

mv:plugType  a            owl:ObjectProperty , rdf:Property ;
        rdfs:comment      "Indicates the type of a plug." ;
        rdfs:domain       mv:Plug ;
        rdfs:isDefinedBy  mv: ;
        rdfs:label        "plug type"@en ;
        rdfs:range        mv:PlugType .

mv:NoParkingAllowed  a    mv:CivicStructureStatus ;
        rdfs:comment      "No parking allowed until the specified time." ;
        rdfs:isDefinedBy  mv: ;
        rdfs:label        "Parken verboten"@de , "No parking allowed"@en .

mv:overnight  a           owl:DatatypeProperty , rdf:Property ;
        rdfs:comment      "Indicates that a time period overnight is possible." ;
        rdfs:domain       mv:TimeSpecification ;
        rdfs:isDefinedBy  mv: ;
        rdfs:label        "über Nacht"@de , "overnight"@en ;
        rdfs:range        xsd:boolean .

mv:vehicleLengthLimitInM
        a                 owl:DatatypeProperty , rdf:Property ;
        rdfs:comment      "Indicates the length limit in meter for vehicles using the parking facility." ;
        rdfs:domain       s:CivicStructure ;
        rdfs:isDefinedBy  mv: ;
        rdfs:label        "Längenbegrenzung für Fahrzeuge"@de , "vehicle length limit"@en ;
        rdfs:range        xsd:decimal .

s:PaymentMethod  a        owl:Class ;
        rdfs:comment      "A payment method is a standardized procedure for transferring the monetary amount for a purchase. Payment methods are characterized by the legal and technical structures used, and by the organization or group carrying out the transaction."@en ;
        rdfs:isDefinedBy  s: ;
        rdfs:label        "Zahlungsart"@de , "Payment method"@en .

mv:DisabledParkingSpace
        a                 mv:ParkingUsageType ;
        rdfs:comment      "Specially designated and identified parking space reserved for persons with disabilities, or in some situations, permission to park in a time-limited space for longer time, or to park at a meter without payment."@en ;
        rdfs:isDefinedBy  mv: ;
        rdfs:label        "Disabled parking space"@en , "Behindertenstellplatz"@de ;
        owl:deprecated    true ;
        skos:note         "Deprecated, use validForUserGroup [a UserGroup] instead." .

mv:AllParkingFacilitiesFull
        a                 mv:CivicStructureStatus ;
        rdfs:comment      "All parking facilities within a specified area are completely occupied."@en ;
        rdfs:isDefinedBy  mv: ;
        rdfs:label        "Alle Parkmöglichkeiten belegt"@de , "All parking facilities full"@en .

mv:AngleParking  a        mv:ArrangementPattern ;
        rdfs:comment      "Bei der Schrägaufstellung wird das Fahrzeug mit einem Aufstellwinkel zwischen 50 und 90 gon (45° und ca. 81°) geparkt. Das Fahrzeug kann vorwärts in den Parkstand einfahren, muss zum Ausparken jedoch wieder rückwärts herausfahren. Diese Aufstellung wird oft bei Parkplätzen verwendet, da sie schmalere Fahrwege als die Senkrechtaufstellung und bessere Platzausnutzung als Parallelaufstellung ermöglicht."@de , "Parking where the parking spaces are arranged at an acute angle to the direction of approach, allowing the driver to enter a space easily and later reverse back out."@en ;
        rdfs:isDefinedBy  mv: ;
        rdfs:label        "Schrägaufstellung"@de , "Angle parking"@en ;
        skos:altLabel     "Echelon parking"@en-uk .

mv:Capacity  a            owl:Class , rdfs:Class ;
        rdfs:comment      "Capacity of a civic structure."@en ;
        rdfs:isDefinedBy  mv: ;
        rdfs:label        "Capacity"@en , "Kapazität"@de .

mv:threePhasedCurrentAvailable
        a                 owl:DatatypeProperty , rdf:Property ;
        rdfs:comment      "Indicates whether three-phased current is available." ;
        rdfs:domain       [ a            owl:Class ;
                            owl:unionOf  ( mv:Plug mv:Charger )
                          ] ;
        rdfs:isDefinedBy  mv: ;
        rdfs:label        "three-phased current available"@en ;
        rdfs:range        xsd:boolean .

mv:cableAvailable  a      owl:DatatypeProperty , rdf:Property ;
        rdfs:comment      "Indicates whether the plug has a cable." ;
        rdfs:domain       mv:Plug ;
        rdfs:isDefinedBy  mv: ;
        rdfs:label        "cable available"@en , "Kabel verfügbar"@de ;
        rdfs:range        xsd:boolean .

mv:customerOf  a          owl:ObjectProperty , rdf:Property ;
        rdfs:comment      "Indicates that a group is customer of a specific business entity."@en ;
        rdfs:domain       mv:UserGroup ;
        rdfs:isDefinedBy  mv: ;
        rdfs:label        "Kunde von"@de , "customer of"@en ;
        rdfs:range        gr:BusinessEntity .

dct:issued  a             owl:AnnotationProperty ;
        rdfs:isDefinedBy  dct: .

mv:ParkingBarrier  a      mv:ParkingFacilityFeature ;
        rdfs:comment      "The parking facility has a parking barrier."@en ;
        rdfs:isDefinedBy  mv: ;
        rdfs:label        "Parkschranke"@de , "Parking barrier"@en .

s:OpeningHoursSpecification
        a                 owl:Class ;
        rdfs:comment      "A structured value providing information about the opening hours of a place or a certain service inside a place."@en ;
        rdfs:isDefinedBy  s: ;
        rdfs:label        "Öffnungszeiten"@de , "Opening hours specification"@en .

mv:connectedTo  a         owl:ObjectProperty , rdf:Property ;
        rdfs:comment      "Indicates the transport connections available." ;
        rdfs:domain       mv:ParkingFacility ;
        rdfs:isDefinedBy  mv: ;
        rdfs:label        "connected to" ;
        rdfs:range        mv:ParkingFacilityConnection .

mv:arrangement  a         owl:ObjectProperty , rdf:Property ;
        rdfs:comment      "Indicates in which pattern a parking space is arranged." ;
        rdfs:domain       mv:ParkingFacility , mv:ParkingSpace ;
        rdfs:isDefinedBy  mv: ;
        rdfs:label        "Anordnung"@de , "arrangement pattern"@en ;
        rdfs:range        mv:ArrangementPattern .

mv:feature  a             owl:ObjectProperty , rdf:Property ;
        rdfs:comment      "Indicates which feature the parking facility provides." ;
        rdfs:domain       mv:ParkingFacility ;
        rdfs:isDefinedBy  mv: ;
        rdfs:label        "feature"@en ;
        rdfs:range        mv:ParkingFacilityFeature .

s:CivicStructure  a       owl:Class ;
        rdfs:comment      "A public structure, such as a town hall or concert hall, parking facility or charging point."@en ;
        rdfs:isDefinedBy  s: ;
        rdfs:label        "Zivile Struktur"@de , "Civic structure"@en ;
        rdfs:subClassOf   s:Place .

mv:numberOfWomensParkingSpaces
        a                 rdf:Property , owl:DatatypeProperty ;
        rdfs:comment      "Indicates the number of women's parking spaces." ;
        rdfs:domain       mv:ParkingFacility ;
        rdfs:isDefinedBy  mv: ;
        rdfs:label        "Anzahl Frauenparkplätze"@de , "number of women's parking spaces"@en ;
        rdfs:range        xsd:integer ;
        owl:deprecated    true ;
        skos:note         "Deprecated, use value of Capacity resource instead." .

mv:Closed  a              mv:CivicStructureStatus ;
        rdfs:comment      "The parking facility is closed." ;
        rdfs:isDefinedBy  mv: ;
        rdfs:label        "Geschlossen"@de , "Closed"@en .

s:PostalAddress  a        owl:Class ;
        rdfs:comment      "The mailing address."@en ;
        rdfs:isDefinedBy  s: ;
        rdfs:label        "Postal address"@en .

mv:IEC_62196_Type_3C  a     mv:PlugType ;
        rdfs:comment        "The type 3A is derived from the Scame charging connectors adding the IEC 62196 pins which is suited for single-phase charging – the connector builds on the experience with the Scame connector for charging of light vehicles (electric motorcycles and scooters). The additional type 3C adds additional 2 pins for three-phase charging for usage at fast charge stations. Based on its origin the connector is sometimes referred to as the Scame type 3 connector." ;
        rdfs:isDefinedBy    mv: ;
        rdfs:label          "SCAME Type 3C"@en ;
        rdfs:seeAlso        <https://en.wikipedia.org/wiki/IEC_62196#Type_3_(EV_Plug_Alliance_connector),_Scame> ;
        mv:ocmConnectionID  "26" ;
        skos:altLabel       "IEC 62196-2 Type 3C" .

mv:numberOfVacantParkingSpaces
        a                 rdf:Property , owl:DatatypeProperty ;
        rdfs:comment      "Indicates the number of vacant parking spaces available." ;
        rdfs:domain       mv:ParkingFacility ;
        rdfs:isDefinedBy  mv: ;
        rdfs:label        "Anzahl freier Stellplätze"@de , "number of vacant parking spaces"@en ;
        rdfs:range        xsd:integer ;
        owl:deprecated    true ;
        skos:note         "Deprecated, use value of Capacity resource instead." .
